\documentclass[12pt]{article}
\usepackage[tmargin=0.5in,bmargin=0.25in]{geometry}
\usepackage{tikz}
\usepackage{multicol}
\usepackage{amsmath, amssymb, amsthm}
\usepackage{enumitem}

\usepackage{tikz}
\usetikzlibrary{automata, positioning}

\title{\vspace{-5ex}CSCI 301 HW 6}
\author{Isaac Boaz}

\begin{document}

\maketitle

\section*{Problem 1}

\begin{enumerate}[label=\alph*.]
    \item \begin{align*}
        S & \rightarrow A \mid B \\
        A & \rightarrow \epsilon \mid aAbb \\
        B & \rightarrow aaab \mid aaaBb
    \end{align*}
    \item \begin{align*}
        S & \rightarrow aAB \\
        A & \rightarrow \epsilon \mid aA  \\
        B & \rightarrow ab \mid aBb
    \end{align*}
    \item \begin{align*}
        S & \rightarrow \epsilon \mid aSb \mid bSa \\
        S & \rightarrow abSba \mid baSab
    \end{align*}
\end{enumerate}

\pagebreak
\section*{Problem 2}
\begin{center}
    \begin{tikzpicture}[shorten >=1pt,node distance=3.5cm,on grid,auto,align=center]
        \node[state,initial,accepting] (q0) {$q_0$};
        \node[state] (q1) [above right=3.5cm and 5cm of q0] {$q_1$};
        \node[state] (q2) [below right=3.5cm and 5cm of q0] {$q_2$};
        \node[state,accepting] (q3) [below right=3.5cm and 5cm of q1] {$q_3$};
        \path[->]
            (q0) edge[above left] node {\(\frac{a, X}{\text{push(} a\text{)}}\)} (q1)
            (q0) edge[below left] node {\(\frac{b, X}{\text{push(} b\text{)}}\)} (q2)
            (q1) edge[loop above] node {\(\frac{a, ?}{\text{push(} a\text{)}}, \frac{b, ?}{\text{pop(}b\text{)}}\)} ()
            (q2) edge[loop below] node {\(\frac{a, ?}{\text{pop(} a\text{)}}, \frac{b, ?}{\text{push(}b\text{)}}\)} ()
            (q1) edge[above right] node {\(\frac{\$, X}{\text{nop}}\)} (q3)
            (q2) edge[below right] node {\(\frac{\$, X}{\text{nop}}\)} (q3);
    \end{tikzpicture}
\end{center}

\pagebreak
\section*{Problem 3}

\begin{tabular}{llc}
\textbf{Derivation} & \textbf{Rule} & \textbf{Lookahead} \\
\hline
\(E \implies TR\) & \(E \rightarrow TR\) & ( \\
\(TR \implies FVR\) & \(T \rightarrow FV\) & ( \\
\(FVR \implies (E)VR\) & \(F \rightarrow (E)\) & ( \\
\((E)VR \implies (TR)VR\) & \(E \rightarrow TR\) & ( \\
\((TR)VR \implies (FVR)VR\) & \(T \rightarrow FV\) & a \\
\((FVR)VR \implies (aVR)VR\) & \(F \rightarrow a\) & a \\
\((aVR)VR \implies (aR)VR\) & \(V \rightarrow \Lambda\) & + \\
\((aR)VR \implies (a+TR)VR\) & \(R \rightarrow +TR\) & + \\
\((a+TR)VR \implies (a+FVR)VR\) & \(T \rightarrow FV\) & a \\
\((a+FVR)VR \implies (a+aVR)VR\) & \(F \rightarrow a\) & a \\
\((a+aVR)VR \implies (a+aR)VR\) & \(V \rightarrow \Lambda\) & ) \\
\((a+aR)VR \implies (a+a)VR\) & \(R \rightarrow \Lambda\) & ) \\
\((a+a)VR \implies (a+a)*FVR\) & \(V \rightarrow *FV\) & * \\
\((a+a)*FVR \implies (a+a)*aVR\) & \(F \rightarrow a\) & a \\
\((a+a)*aVR \implies (a+a)*aR\) & \(V \rightarrow \Lambda\) & \$ \\
\((a+a)*aR \implies (a+a)*a\) & \(R \rightarrow \Lambda\) & \$ \\
\end{tabular}

\end{document}
